generic/Zeta.MultiSetHashDomain.fsti
@@ -1,0 +1,21 @@
+module Zeta.MultiSetHashDomain
+
+open FStar.BitVector
+open Zeta.App
+open Zeta.Key
+open Zeta.MultiSet
+open Zeta.Record
+open Zeta.Thread
+open Zeta.Time
+
+type ms_hashfn_dom (aprm: app_params) =
+  | MHDom: r:record aprm -> t:timestamp -> tid:thread_id -> ms_hashfn_dom aprm
+
+val ms_hashfn_dom_cmp (aprm: app_params)
+  : cmp (ms_hashfn_dom aprm)
+
+type mset_ms_hashfn_dom (aprm: app_params) = mset (ms_hashfn_dom aprm) (ms_hashfn_dom_cmp aprm)
+
+let epoch #aprm (e: ms_hashfn_dom aprm) =
+  let MkTimestamp e _ = e.t in
+  e
